src/Operational_Semantics.thy
@@ -11,33 +11,58 @@ record 'a node_state =
   document     :: json_document
   vars         :: "('a, json_cursor) alist"
   highest_seen :: "nat"
+  program      :: "'a program"
 
 definition valid_node_state :: "'a node_state \<Rightarrow> bool" where
   "valid_node_state \<sigma> \<equiv> \<forall>v c. DAList.lookup (vars \<sigma>) v = Some c \<longrightarrow> document \<sigma> \<bowtie> c"
 
-definition initial_node_state :: "'a node_state" where
-  "initial_node_state \<equiv>
+definition load :: "'a program \<Rightarrow> 'a node_state" where
+  "load \<pi> \<equiv>
      \<lparr> document     = Map_Node DAList.empty
      , vars         = DAList.empty
      , highest_seen = 0
+     , program      = \<pi>
      \<rparr>"
+
+definition next_command :: "'a node_state \<Rightarrow> ('a cmd \<times> 'a node_state) option" where
+  "next_command n \<equiv>
+     case (program n) of
+       []   \<Rightarrow> None
+     | x#xs \<Rightarrow> Some (x, n\<lparr> program := xs \<rparr>)"
 
 definition generate_operation_id :: "'a node_state \<Rightarrow> nat \<Rightarrow> (lamport \<times> 'a node_state)" where
   "generate_operation_id \<A> ident \<equiv>
      let c = Suc (highest_seen \<A>);
          a = \<A>\<lparr> highest_seen := c \<rparr>
-     in ((c, ident), a)"
+     in (OperationID (c, ident), a)"
 
 lemma initial_node_state_valid [simp]:
-  shows "valid_node_state initial_node_state"
-by (auto simp add: valid_node_state_def initial_node_state_def)
+  shows "valid_node_state (load \<pi>)"
+by (auto simp add: valid_node_state_def load_def)
+
+fun next_list_element :: "('a \<times> lamport) list \<Rightarrow> lamport \<Rightarrow> lamport option" where
+  "next_list_element []       l = None" |
+  "next_list_element [(v, k)]      Head = Some k" |
+  "next_list_element [x]      (OperationID k) = None" |
+  "next_list_element ((v,k)#y#xs) Head = Some k" |
+  "next_list_element ((v,k')#y#xs) (OperationID k) =
+     (if OperationID k = k' then
+        Some (snd y)
+      else next_list_element (y#xs) (OperationID k))"
                                                                          
 inductive expr_operational_semantics :: "'a node_state \<Rightarrow> 'a expr \<Rightarrow> json_cursor \<Rightarrow> bool" ("_/ \<turnstile>/ _/ \<longlonglongrightarrow>e/ _" [65,65,65]65) where
   expr_operational_semantics_Doc [intro!]: "\<A> \<turnstile> doc \<longlonglongrightarrow>e Cursor []" |
   expr_operational_semantics_Var [intro!]: "\<lbrakk> DAList.lookup (vars \<A>) v = Some c \<rbrakk> \<Longrightarrow> \<A> \<turnstile> v\<acute> \<longlonglongrightarrow>e c" |
   expr_operational_semantics_Lookup [intro!]: "\<lbrakk> \<A> \<turnstile> e \<longlonglongrightarrow>e c; c' = grow_map_entry c k \<rbrakk> \<Longrightarrow> \<A> \<turnstile> e\<lbrakk> k \<rbrakk> \<longlonglongrightarrow>e c'" |
-  expr_operational_semantics_Iter [intro!]: "\<lbrakk> \<A> \<turnstile> e \<longlonglongrightarrow>e c; c' = grow_list_entry c 0 \<rbrakk> \<Longrightarrow> \<A> \<turnstile> e\<cdot>iter \<longlonglongrightarrow>e c'" |
-  expr_operational_semantics_Next [intro!]: "\<lbrakk> \<A> \<turnstile> e \<longlonglongrightarrow>e c; c = Cursor cs; cs \<noteq> []; last cs = ListC k; c' = Cursor (butlast cs #> ListC (Suc k)); document \<A> \<bowtie> c' \<rbrakk> \<Longrightarrow> \<A> \<turnstile> e\<cdot>next \<longlonglongrightarrow>e c'"
+  expr_operational_semantics_Iter [intro!]: "\<lbrakk> \<A> \<turnstile> e \<longlonglongrightarrow>e c; c' = grow_list_entry c Head \<rbrakk> \<Longrightarrow> \<A> \<turnstile> e\<cdot>iter \<longlonglongrightarrow>e c'" |
+  expr_operational_semantics_Next [intro!]: "\<lbrakk> \<A> \<turnstile> e \<longlonglongrightarrow>e c; c = Cursor cs; cs \<noteq> []; last cs = ListC k; Some (List_Node js) = fetch (document \<A>) (Cursor (butlast cs));
+                                               Some c' = next_list_element js k; c'' = Cursor (butlast cs #> ListC c'); document \<A> \<bowtie> c'' \<rbrakk> \<Longrightarrow> \<A> \<turnstile> e\<cdot>next \<longlonglongrightarrow>e c''"
+
+definition from_list_node :: "json_document \<Rightarrow> (json_document \<times> lamport) list option" where
+  "from_list_node j \<equiv>
+     case j of
+       List_Node js \<Rightarrow> Some js
+     | _ \<Rightarrow> None"
 
 fun execute_expr :: "'a node_state \<Rightarrow> 'a expr \<rightharpoonup> json_cursor" where
   "execute_expr \<A> Doc     = Some (Cursor [])" |
@@ -48,7 +73,7 @@ fun execute_expr :: "'a node_state \<Rightarrow> 'a expr \<rightharpoonup> json_
         }" |
   "execute_expr \<A> (Iter e) =
      do { c \<leftarrow> execute_expr \<A> e
-        ; Some (grow_list_entry c 0)
+        ; Some (grow_list_entry c Head)
         }" |
   "execute_expr \<A> (Next e) =
      do { c \<leftarrow> execute_expr \<A> e
@@ -59,10 +84,14 @@ fun execute_expr :: "'a node_state \<Rightarrow> 'a expr \<rightharpoonup> json_
               else
                 (case last cs of
                    ListC k \<Rightarrow>
-                     let c' = Cursor (butlast cs #> ListC (Suc k)) in
-                       if json_document_cursor_compatible (document \<A>) c' then
-                         Some c'
-                       else None
+                     do { js \<leftarrow> fetch (document \<A>) (Cursor (butlast cs))
+                        ; js \<leftarrow> from_list_node js
+                        ; c' \<leftarrow> next_list_element js k
+                        ; let c'' = Cursor (butlast cs #> ListC c')
+                        ; if json_document_cursor_compatible (document \<A>) c'' then
+                            Some c''
+                          else None
+                        }
                  | _ \<Rightarrow> None)
         }"
 
@@ -103,7 +132,7 @@ next
     by fastforce
   hence "\<A> \<turnstile>e \<longlonglongrightarrow>e c'"
     using IH by simp
-  have "c = grow_list_entry c' 0"
+  have "c = grow_list_entry c' Head"
     using * ** by simp
   thus "\<A> \<turnstile> e\<cdot>iter \<longlonglongrightarrow>e c"
     using `\<A> \<turnstile>e \<longlonglongrightarrow>e c'` by auto
@@ -122,53 +151,100 @@ next
     apply(case_tac "x = []"; simp)
     apply(case_tac "last x"; simp add: Let_def)
     done
-  from this and * ** have 3: "c' = Cursor (butlast cs #> ListC (Suc k))"
-    apply(simp only: execute_expr.simps)
-    apply(cases "execute_expr \<A> e"; simp)
+  from * ** and this obtain js where 3: "Some (List_Node js) = fetch (document \<A>) (Cursor (butlast cs))"
+    apply simp
+    apply(case_tac "execute_expr \<A> e"; simp)
     apply(case_tac "a"; simp)
-    apply(case_tac "x = []"; simp)
-    apply(case_tac "last x"; simp add: Let_def)
-    apply(case_tac "json_document_cursor_compatible (document \<A>) (Cursor (butlast x #> ListC (Suc x1)))"; simp)
+    apply(case_tac "x=[]"; simp)
+    apply(case_tac "last x"; simp)
+    apply(case_tac "fetch (document \<A>) (Cursor (butlast x))"; simp)
+    apply(case_tac "from_list_node aa"; simp)
+    apply(case_tac "next_list_element ab x1"; simp add: Let_def)
+    apply(case_tac "json_document_cursor_compatible (document \<A>) (Cursor (butlast x #> ListC ac))"; simp)
+    apply(case_tac aa; simp add: from_list_node_def)
     done
-  from this and * ** have 4: "document \<A> \<bowtie> c'"
-    apply(simp only: execute_expr.simps bind.simps)
-    apply(case_tac "c"; simp)
-    apply(case_tac "x = []"; simp)
-    apply(case_tac "last x"; simp add: Let_def)
-    apply(case_tac "json_document_cursor_compatible (document \<A>) (Cursor (butlast x #> ListC (Suc x1)))"; simp)
-    apply(simp add: json_document_cursor_compatible_sound)
+  from * ** and 2 3 obtain c'' where 4: "Some c'' = next_list_element js k"
+    apply simp
+    apply(case_tac "execute_expr \<A> e"; simp)
+    apply(case_tac "a"; simp)
+    apply(case_tac "x=[]"; simp)
+    apply(case_tac "last x"; simp)
+    apply(case_tac "fetch (document \<A>) (Cursor (butlast x))"; simp)
+    apply(case_tac "from_list_node aa"; simp)
+    apply(case_tac "next_list_element ab x1"; simp add: Let_def)
+    apply(case_tac "json_document_cursor_compatible (document \<A>) (Cursor (butlast x #> ListC ac))"; simp)
+    apply(simp add: from_list_node_def)
+    apply(case_tac "aa"; simp)
+    done
+  from * ** and 2 3 4 have 5: "c' = Cursor (butlast cs #> ListC c'')"
+    apply simp
+    apply(case_tac "execute_expr \<A> e"; simp)
+    apply(case_tac "a"; simp)
+    apply(case_tac "x=[]"; simp)
+    apply(case_tac "last x"; simp)
+    apply(case_tac "fetch (document \<A>) (Cursor (butlast x))"; simp)
+    apply(case_tac "from_list_node aa"; simp)
+    apply(case_tac "next_list_element ab x1"; simp add: Let_def)
+    apply(case_tac "json_document_cursor_compatible (document \<A>) (Cursor (butlast x #> ListC ac))"; simp)
+    apply(simp add: from_list_node_def)
+    apply(case_tac "aa"; simp)
+    done
+  from * have 6: "document \<A> \<bowtie> c'"
+    apply simp
+    apply(case_tac "execute_expr \<A> e"; simp)
+    apply(case_tac "a"; simp)
+    apply(case_tac "x=[]"; simp)
+    apply(case_tac "last x"; simp)
+    apply(case_tac "fetch (document \<A>) (Cursor (butlast x))"; simp)
+    apply(case_tac "from_list_node aa"; simp)
+    apply(case_tac "next_list_element ab x1"; simp add: Let_def)
+    apply(case_tac "json_document_cursor_compatible (document \<A>) (Cursor (butlast x #> ListC ac))"; simp)
+    apply(rule json_document_cursor_compatible_sound, assumption)
     done
   thus "\<A> \<turnstile> e\<cdot>next \<longlonglongrightarrow>e c'"
-    using 1 2 3 by auto
+    using 1 2 3 4 5 by auto
 qed
 
 lemma execute_expr_sound_complete:
   assumes "\<A> \<turnstile> e \<longlonglongrightarrow>e c"
   shows   "execute_expr \<A> e = Some c"
-using assms by(induction rule: expr_operational_semantics.induct, auto simp add: json_document_cursor_compatible_complete)
+using assms
+  apply(induction rule: expr_operational_semantics.induct; simp)
+  apply(case_tac "fetch (document \<A>') (Cursor (butlast cs))"; simp)
+  apply(case_tac "a"; simp add: from_list_node_def)
+  apply(case_tac "next_list_element x2 k"; simp add: Let_def)
+  apply(rule json_document_cursor_compatible_complete, assumption)
+done
 
-definition json_document_of_val :: "val \<Rightarrow> json_document" where
-  "json_document_of_val v \<equiv>
+definition singleton_alist :: "'a \<Rightarrow> 'b \<Rightarrow> ('a, 'b) alist" where
+  "singleton_alist k v \<equiv> DAList.update k v (DAList.empty)"
+
+definition json_document_of_val :: "val \<Rightarrow> lamport \<Rightarrow> json_document" where
+  "json_document_of_val v l \<equiv>
      case v of
-       val.Int i \<Rightarrow> Leaf (primitive.Int i)
-     | val.String s \<Rightarrow> Leaf (primitive.String s)
-     | val.Bool b \<Rightarrow> Leaf (primitive.Bool b)
-     | val.Null \<Rightarrow> Leaf primitive.Null
+       val.Int i \<Rightarrow> Leaf (singleton_alist l (primitive.Int i))
+     | val.String s \<Rightarrow> Leaf (singleton_alist l (primitive.String s))
+     | val.Bool b \<Rightarrow> Leaf (singleton_alist l (primitive.Bool b))
+     | val.Null \<Rightarrow> Leaf (singleton_alist l primitive.Null)
      | val.Empty_Map \<Rightarrow> Map_Node DAList.empty
      | val.Empty_List \<Rightarrow> List_Node []"
 
-definition assign :: "json_document \<Rightarrow> json_cursor \<Rightarrow> val \<rightharpoonup> json_document" where
+definition assign :: "json_document \<Rightarrow> json_cursor \<Rightarrow> (val \<times> lamport) \<rightharpoonup> json_document" where
   "assign j c v \<equiv>                                      
-     edit j c (\<lambda>_. Some (json_document_of_val v)) (json_document_of_val v)"
+     edit j c (\<lambda>_. Some (json_document_of_val (fst v) (snd v))) (json_document_of_val (fst v) (snd v))"
 
-inductive cmd_operation_semantics :: "'a node_state \<Rightarrow> 'a cmd \<Rightarrow> 'a node_state \<Rightarrow> bool" ("_/ \<turnstile>/ _/ \<longlonglongrightarrow>c/ _" [65,65,65]65) where
-  "\<lbrakk> \<A> \<turnstile> c \<longlonglongrightarrow>c \<A>'; \<A>' \<turnstile> d \<longlonglongrightarrow>c \<A>'' \<rbrakk> \<Longrightarrow> \<A> \<turnstile> (c \<triangleright> d) \<longlonglongrightarrow>c \<A>''" |
-  "\<lbrakk> \<A> \<turnstile> e \<longlonglongrightarrow>e c; \<A>' = \<A>\<lparr> vars := DAList.update x c (vars \<A>) \<rparr> \<rbrakk> \<Longrightarrow> \<A> \<turnstile> (let x\<acute> \<Leftarrow> e) \<longlonglongrightarrow>c \<A>'" |
-  "\<lbrakk> \<A> \<turnstile> e \<longlonglongrightarrow>e c; Some d = assign (document \<A>) c v; \<A>' = \<A>\<lparr> document := d \<rparr> \<rbrakk> \<Longrightarrow> \<A> \<turnstile> e \<Leftarrow> v \<longlonglongrightarrow>c \<A>'" |
-  "\<lbrakk> \<A> \<turnstile> e \<longlonglongrightarrow>e c; Some d = insert (document \<A>) c (json_document_of_val v); \<A>' = \<A>\<lparr> document := d \<rparr> \<rbrakk> \<Longrightarrow> \<A> \<turnstile> e\<cdot>insert\<lparr> v \<rparr> \<longlonglongrightarrow>c \<A>'"
+inductive cmd_operation_semantics :: "'a node_state \<Rightarrow> nat \<Rightarrow> 'a cmd \<Rightarrow> 'a node_state \<Rightarrow> bool" ("_\<langle>_\<rangle>/ \<turnstile>/ _/ \<longlonglongrightarrow>c/ _" [65,65,65,65]65) where
+  "\<lbrakk> \<A> \<turnstile> e \<longlonglongrightarrow>e c; \<A>' = \<A>\<lparr> vars := DAList.update x c (vars \<A>) \<rparr> \<rbrakk> \<Longrightarrow> \<A>\<langle>m\<rangle> \<turnstile> (let x\<acute> \<Leftarrow> e) \<longlonglongrightarrow>c \<A>'" |
+  "\<lbrakk> \<A> \<turnstile> e \<longlonglongrightarrow>e c; (lamport, \<A>') = generate_operation_id \<A> m; Some d = assign (document \<A>') c (v, lamport); \<A>'' = \<A>'\<lparr> document := d \<rparr> \<rbrakk> \<Longrightarrow> \<A>\<langle>m\<rangle> \<turnstile> e \<Leftarrow> v \<longlonglongrightarrow>c \<A>''" |
+  "\<lbrakk> \<A> \<turnstile> e \<longlonglongrightarrow>e c; (lamport, \<A>') = generate_operation_id \<A> m; Some d = insert (document \<A>') c ((json_document_of_val v lamport), lamport); \<A>'' = \<A>'\<lparr> document := d \<rparr> \<rbrakk> \<Longrightarrow> \<A>\<langle>m\<rangle> \<turnstile> e\<cdot>insert\<lparr> v \<rparr> \<longlonglongrightarrow>c \<A>''"
+
 (*
   "\<lbrakk> \<A> \<turnstile> e \<longlonglongrightarrow>e c \<rbrakk> \<Longrightarrow> \<A> \<turnstile> e\<cdot>delete \<longlonglongrightarrow>c undefined" |
   "\<A> \<turnstile> yield \<longlonglongrightarrow>c undefined"
 *)
+
+inductive concurrent_node_semantics :: "'a node_state list \<Rightarrow> 'a node_state list \<Rightarrow> bool" ("_/ \<leadsto>/ _" [65]65) where
+  "\<lbrakk> i < length \<A>s; (lt, \<A>, gt) = split_at \<A>s i; Some (c, \<A>') = next_command \<A>; \<A>'\<langle>i\<rangle> \<turnstile> c \<longlonglongrightarrow>c \<A>''; \<A>s' = lt @ [\<A>''] @ gt \<rbrakk> \<Longrightarrow> \<A>s \<leadsto> \<A>s'" |
+  "\<lbrakk> \<A>s \<leadsto> \<A>s'; \<A>s' \<leadsto> \<A>s'' \<rbrakk> \<Longrightarrow> \<A>s \<leadsto> \<A>s''"
 
 end
